agents/wasmspec/log.md
@@ -1962,3 +1962,4 @@ test_write
 
 2026-03-24T23:15:01+00:00 SKIP: already running
 2026-03-25T00:15:01+00:00 SKIP: already running
+2026-03-25T00:54:43+00:00 DONE
